src/variability_test.lean
@@ -1,0 +1,70 @@
+-- variability_test.lean
+-- testing the variability module
+import data.set tactic data.setoid.partition  data.finset
+import .variability
+
+open variability
+
+-- the auto-derive works only when data.set and tactic are imported
+@[derive [fintype, decidable_eq]] inductive Features 
+| Feat_A
+| Feat_B
+| Feat_C
+
+open Features
+instance : has_to_string Features :=
+⟨λ f, match f with
+      | Feat_A := "Feat_A"
+      | Feat_B := "Feat_B"
+      | Feat_C := "Feat_C"
+      end⟩
+
+instance : has_repr Features := ⟨to_string⟩
+
+def T : Type := finset Features
+def x : T := {Feat_A}
+
+def p : SPL := ⟨Features⟩
+
+def pc₁ : PC := FeatureExpr.Atom Features.Feat_A
+def pc₂ : PC := FeatureExpr.Not pc₁
+def pc₃ := FeatureExpr.Atom Feat_B
+def pc₄ := FeatureExpr.And pc₁ pc₃
+def pc₅ := FeatureExpr.Or pc₁ pc₂
+
+def s₁ := semantics pc₁
+def s₂ := semantics pc₂
+
+
+#eval s₁
+#eval s₂
+
+open setoid
+
+#eval (semantics pc₄)
+#eval (semantics pc₅)
+
+#eval (checkDisj (list.map semantics [pc₁, pc₂]))
+#eval (checkTotal [pc₁, pc₂])
+def p₁ : ConfigPartition := {ConfigPartition . pcs := [pc₁, pc₂]}
+
+#eval (checkDisj (list.map semantics [pc₁, pc₃]))
+#eval (checkTotal [pc₁, pc₃])
+
+
+-- should fail
+--def p₁ : ConfigPartition := {ConfigPartition . pcs := [pc₁, pc₃]}
+
+def v₁ : Var := Var.mk [(7,pc₁), (3,pc₂)]
+#eval v₁
+
+#eval index {Feat_B} v₁
+#eval index {Feat_C} v₁
+#eval index {Feat_A} v₁
+
+-- should fail
+--def v₂ : Var := Var.mk [(7,pc₁), (3,pc₃)]
+
+#eval p₁
+#eval (to_bool (is_eqv p₁ {Feat_B} {Feat_C}))
+#eval (is_eqv p₁ {Feat_B} {Feat_A})
